WIP: debug

dataplane/Examples/Batch_op_Correctness.thy
@@ -6,7 +6,9 @@ imports
   Ooo_Input_op
   Batch_op
   "../MyProduct_Instances"
+  "../AntichainOrder"
 begin
+
 
 partial_function (llist) batch_fun_spec where
  "batch_fun_spec f lxs buf caps = (case lxs of
@@ -29,11 +31,12 @@ abbreviation "t1 \<equiv> MyPair (Suc 0) (0 :: nat)"
 abbreviation "t2 \<equiv> MyPair (0 :: nat) (Suc 0)"
 abbreviation "t3 \<equiv> MyPair (Suc 0) (Suc 0)"
 
-abbreviation "inps1 \<equiv> llist_of [Data 1 4, Data (0 :: nat) (10 :: nat), Data 0 0, Data 2 11]"
+term DEBUG
+
+abbreviation "inps1 \<equiv> llist_of [Data (0 :: nat) (0 :: nat)]"
 
 abbreviation "inps2 \<equiv> llist_of [Mint t1, Mint t2, Mint t3, Data t3 10, Drop t3, Data t2 7, Data t1 (-2 :: int), Data t2 (-1), Data t1 (- 3), Drop t1, Drop t2]"
 
-value \<open>list_of (lconcat (batch_fun_spec (\<lambda> b. [Max (set b)]) inps1 [] []))\<close>
 value \<open>list_of (lconcat (batch_fun_spec (\<lambda> b. [Max (set b)]) inps1 [] []))\<close>
 
 value \<open>list_of (lconcat (batch_fun_spec (\<lambda> b. [Max (set b)]) inps2 [] []))\<close>
@@ -47,7 +50,7 @@ abbreviation init_input_state where
    input = (\<lambda> _. []),
    outpu = (\<lambda> _. []),
    front = undefined,
-   ocaps = (\<lambda> _. [0]),
+   ocaps = (\<lambda> _. [\<bottom>]),
    initia = False,
    en1 = Inl,
    de1 = projl,
@@ -64,7 +67,7 @@ abbreviation init_operator_state_ty2 where
    input = (\<lambda> _. []),
    outpu = (\<lambda> _. []),
    front = undefined,
-   ocaps = (\<lambda> _. [0]),
+   ocaps = (\<lambda> _. [\<bottom>]),
    initia = False,
    en1 = Inl,
    de1 = projl,
@@ -73,7 +76,9 @@ abbreviation init_operator_state_ty2 where
    \<rparr>"
 abbreviation "l2 \<equiv> Logic (batch_fun_op (init_operator_state_ty2 default_internal_summary) (\<lambda> b. if b = [] then [] else [Max (set b)])) default_internal_summary"
 
-abbreviation "dt \<equiv> compile_dataflow (Comp [(0, 1) \<mapsto> (0, 1)] (l1 (\<lambda> _. inps1)) l2) :: (1 \<times> 1, 1 \<times> 1, (nat + nat) \<times> nat) op"
+abbreviation "main_dt \<equiv> Comp [(0, 1) \<mapsto> (0, 1)] (l1 (\<lambda> _. inps1)) l2"
+
+abbreviation "dt \<equiv> compile_dataflow main_dt :: (2 \<times> 1, 2 \<times> 1, (nat + nat) \<times> nat) op"
 
 lemma one_minus[code]:
   "(1 :: 1) - x = 1"
@@ -81,10 +86,6 @@ lemma one_minus[code]:
 lemma one_plus[code]:
   "(1 :: 1) + x = 1"
   by auto
-
-find_theorems eval'
-
-find_theorems cset_of_llist cUnion
 
 partial_function (llist) lrmdups_aux where
   "lrmdups_aux f S lxs = (case lxs of LNil \<Rightarrow> LNil | LCons x lxs \<Rightarrow> (if f x \<in> S then lrmdups_aux f S lxs else LCons x (lrmdups_aux f (insert (f x) S) lxs)))"
@@ -94,9 +95,6 @@ definition "lrmdups f = lrmdups_aux f {}"
 
 definition "compress_cfilter P xs = cfilter P xs"
 
-lemma compress_cfilter_code[code]: "compress_cfilter P (cset_of_llist xs) = cfilter P (cset_of_llist (lrmdups id xs))"
-  sorry
-
 friend_of_corec lappend where
   "lappend xs lys = (case xs of LNil \<Rightarrow> (case lys of LNil \<Rightarrow> LNil | LCons x xs \<Rightarrow> LCons x xs)
     | LCons x xs \<Rightarrow> LCons x (lappend xs lys))"
@@ -105,8 +103,8 @@ friend_of_corec lappend where
   done
 
 
-definition "my_eval = compress_cfilter ((\<noteq>) [])(eval 18 dt)"
-value [GHC] "my_eval" 
+(* definition "my_eval = compress_cfilter ((\<noteq>) [])(eval 18 dt)"
+value [GHC] "my_eval"  *)
  
 definition "my_check = approx_in 20 [VOut (1, 1) (Inr 4, 1), VOut (1, 1) (Inr 10, 0)] dt"
 (* 
@@ -119,46 +117,146 @@ definition "rmdup_traces xs = xs"
 
 abbreviation "flat_choices ops \<equiv> cUnion (cimage choices ops)"
 
-find_consts "_ cset"
+abbreviation "is_Visible x \<equiv> is_Write x \<or> is_Read x"
 
 context includes cset.lifting begin
 lift_definition ccard :: "'m cset \<Rightarrow> nat" is card .
 end
 
-term the_enat
-
 lemma ccard_code[code]:
   "ccard (cset_of_llist xs) = the_enat (llength xs)"
   sorry
-abbreviation "is_Visible x \<equiv> is_Write x \<or> is_Read x"
 
 abbreviation "optm ops \<equiv> let ops' = (cfilter (is_Visible o snd) ops) in if ccard ops' > 0 then ops' else ops"
+
+code_printing
+  type_constructor llist \<rightharpoonup>
+    (Haskell) "![(_)]"
+  | constant LNil \<rightharpoonup>
+    (Haskell) "[]"
+  | constant LCons \<rightharpoonup>
+    (Haskell) infix 5 ":"
+  | class_instance llist :: equal \<rightharpoonup>
+    (Haskell) -
+  | constant "HOL.equal :: 'a llist \<Rightarrow> 'a llist \<Rightarrow> bool" \<rightharpoonup>
+    (Haskell) infix 4 "=="
+  | constant "lappend" \<rightharpoonup>
+    (Haskell) infixr 5 "++"
+  | constant lmap \<rightharpoonup>
+    (Haskell) "map"
+  | constant lfilter \<rightharpoonup>
+    (Haskell) "filter"
+  | constant lconcat \<rightharpoonup>
+    (Haskell) "Prelude.concat"
+  | constant lhd \<rightharpoonup>
+    (Haskell) "Prelude.head"
+  | constant hd \<rightharpoonup>
+    (Haskell) "Prelude.head"
+  | constant ltl \<rightharpoonup>
+    (Haskell) "Prelude.tail"
+  | constant tl \<rightharpoonup>
+    (Haskell) "Prelude.tail"
+  | constant lzip \<rightharpoonup>
+    (Haskell) "zip"
+  | constant llist.lnull \<rightharpoonup>
+    (Haskell) "null"
+  | constant ltakeWhile \<rightharpoonup>
+    (Haskell) "takeWhile"
+  | constant ldropWhile \<rightharpoonup>
+    (Haskell) "dropWhile"
+  | constant llist_all \<rightharpoonup>
+    (Haskell) "all"
+  | constant llist_of \<rightharpoonup>
+    (Haskell) "id"
+
+definition "csetid (xs :: 'm cset) = xs"
+
+code_printing code_module "Cset" \<rightharpoonup> (Haskell)
+  \<open>module Cset (foo, Cset (..) ) where
+newtype Cset a = Cset [a];
+
+foo (Cset []) = Cset [];
+foo (Cset xs) = Cset [Prelude.head xs];
+
+\<close> 
+
+code_printing
+  type_constructor cset \<rightharpoonup>
+    (Haskell) "Cset.Cset _"
+  | constant cset_of_llist \<rightharpoonup>
+    (Haskell) "Cset.Cset"
+  | constant csetid \<rightharpoonup>
+    (Haskell) "Cset.foo"
+
+term choice5
+lemma choice5_code[code]:
+  "choice5 op1 op2 op3 op4 op5 = Choice {||}"
+  sorry
 
 fun fast_eval' :: "nat \<Rightarrow> _ \<Rightarrow> _ \<Rightarrow> ('i, 'o, 'd :: {countable}) op \<Rightarrow> (('i, 'o, 'd) VIO list \<times> ('i, 'o, 'd) op) cset"  where
   "fast_eval' 0 m i op = {|([], op)|}"
 | "fast_eval' n m 0 op = {||}"
-| "fast_eval' (Suc n) m i (Write op p x) = cimage (\<lambda>(t, op). (VOut p x # t, op)) (fast_eval' n m m op)"
-| "fast_eval' (Suc n) m i (Read p f) = cUnion (cimage (\<lambda>x. cimage (\<lambda>(t, op). (VInp p x # t, op)) (fast_eval' n m m (f x))) (cUNIV :: 'd cset))"
+| "fast_eval' (Suc n) m i (Write op p x) = (cimage (\<lambda>(t, op). (VOut p x # t, op)) (fast_eval' n m m op))"
+| "fast_eval' (Suc n) m i (Read p f) = (cUnion (cimage (\<lambda>x. cimage (\<lambda>(t, op). (VInp p x # t, op)) (fast_eval' n m m (f x))) (cUNIV :: 'd cset)))"
 | "fast_eval' n m (Suc i) (Silent op) = (cimage (\<lambda>(t, op). (t, op)) (fast_eval' n m i op))"
-| "fast_eval' n m (Suc i) (Choice ops) = (if ops = {||} then {|([], \<oslash>)|} else (let ops' = cUnion (cimage (fast_eval' n m i) ops) in optm ops'))"
+| "fast_eval' n m (Suc i) (Choice ops) = (
+  if ops = {||} then {|([], \<oslash>)|} else
+ (let ops' = (cUnion (cimage (fast_eval' n m i) ops)) in if ops' = {||} then {||} else ops'))"
 
-definition "fast_eval n m op = cimage fst (fast_eval' n m m op)"
-
-
-definition "my_fast_eval = compress_cfilter ((\<noteq>) []) (fast_eval 1 14 dt)"
-value [GHC] "my_fast_eval" 
-
-definition "fast_approx_in n m pfx op = 
-  (\<not> cis_empty (cfilter (\<lambda>xs. Sublist.prefix pfx xs) (cimage fst (fast_eval' n m m op))))"
-
-definition "my_fast_check = fast_approx_in 3 14 [VOut (1, 1) (Inr 4, 1), VOut (1, 1) (Inr 10, 0), VOut (1, 1) (Inr 11, 2)] dt"
-
-value [GHC] "my_fast_check" 
+definition "fast_eval n m op = (cfilter ((\<noteq>) []) (cimage fst ((fast_eval' n m m op))))"
 
 
-(* export_code my_test in Haskell 
-  module_name Test
+definition "my_fast_eval = cimage (map (\<lambda> (d, t). (projr d, t)) o  map vdata) (fast_eval 1 20 dt)"
+
+
+term DEBUG
+
+value [GHC] my_fast_eval
+
+
+
+
+
+
+definition safe_cthe_elem where "safe_cthe_elem C = (if C = {||} then None else Some (cthe_elem C))"
+
+
+lemma safe_cthe_elem_code[code]:
+  "safe_cthe_elem (cset_of_llist xs) = Some (lhd xs)"
+  sorry
+
+(* lemma cthe_elem_code[code]:
+  "cthe_elem (cset_of_llist xs) = Set.the_elem (lset xs)"
+  apply transfer
+  apply auto
+  done *)
+
+fun hd_in_traces where
+  "hd_in_traces n (Write op p x) = (Some ((VOut p x), op))"
+| "hd_in_traces n (Read p f) = (Some ((VInp p undefined), f undefined))"
+| "hd_in_traces (Suc n) (Silent op) = hd_in_traces n op"
+| "hd_in_traces (Suc n) (Choice ops) = 
+  (let ops' = cimage the (cfilter ((\<noteq>) None) (cimage (hd_in_traces n) ops)) in
+  (if ops' = {||} then None else safe_cthe_elem ops'))"
+| "hd_in_traces 0 op = None"
+
+fun in_traces where
+  "in_traces 0 op i = []"
+| "in_traces (Suc n) op i = (case hd_in_traces i op of None \<Rightarrow> [] | Some (io, op') \<Rightarrow> io # in_traces n op' i)"
+
+definition "my_fast_check3 = in_traces 1 dt 10"
+
+(* 
+value [GHC] "my_fast_check3"
+
  *)
+
+
+  export_code safe_cthe_elem in Haskell 
+  module_name Test26
+
+end
+
 
 abbreviation "inp_op os \<equiv> map_op (case_option (Inl (0 :: 2)) (\<lambda> p. Inr (0, p))) (case_option (Inl (0 :: 2)) (\<lambda> p. Inr (0, p))) (ooo_input_op {|1|} os)"
 abbreviation "bt_op os f \<equiv> map_op (case_option (Inl (1 :: 2)) (\<lambda> p. Inr (1, p))) (case_option (Inl (1 :: 2)) (\<lambda> p. Inr (1, p))) (batch_fun_op os f)"
@@ -167,25 +265,48 @@ abbreviation "inp_bt_op os1 cbuf os2 f \<equiv>
    map_op (case_sum id id) (case_sum id id)
    (comp_op [Inr (0 :: 2, 0 :: 1) \<mapsto> Inr (1 :: 2, 0 :: 1)] cbuf (inp_op (os1\<lparr> en1 := Inl \<rparr>)) (bt_op (os2\<lparr> de1 := projl, en2 := Inr \<rparr>) f))"
 
+
+definition \<open>subgraph_inv dtt cgs c = (let (su, _) = compile_dataflow_tree dtt in
+ \<lparr> pt_tr = change_multiplicities su cgs c,
+   edges = (\<lambda> l1. [l2 \<leftarrow> Enum.enum. \<not> is_empty_antichain (su l1 l2) \<and> is_Src (port l1) \<and> is_Trg (port l2) ]),
+   summ = su \<rparr>)\<close>
+
+
+
+term "[Inr (0 :: 2, 0 :: 1) \<mapsto> Inr (1 :: 2, 0 :: 1)]"
+
 lemma dataflow_op_inp_bt_op_wbisim_source_op_aux:
-  fixes lxs :: \<open>('t :: {ccompare,canonically_ordered_monoid_add,ordered_ab_semigroup_monoid_add_imp_le}, 'd1) event llist\<close>
+  fixes lxs :: \<open>('t :: {ccompare,canonically_ordered_monoid_add,ordered_ab_semigroup_monoid_add_imp_le,bot}, 'd1) event llist\<close>
   and f :: \<open>'d1 buf \<Rightarrow> 'd2 buf\<close>
   and os1 :: \<open>(1, 'd1 + 'd2, 'd1, 't) input_state\<close>
   and os2 :: \<open>(1, 'd1 + 'd2, 'd1, 'd2, 't) operator_state_ty2\<close>
 assumes
-  state_inv: 
-   \<open>es os1 1 = lxs\<close>
-   \<open>outpu os1 1 = map (\<lambda> (d, t). (Inl d, t)) outpos1\<close>
-   \<open>input os2 1 = map (\<lambda> (d, t). (Inl d, t)) inpos2\<close>
-   \<open>buf = outpos1 @ cbuf @ inpos\<close>
+  buffers_inv: 
+  \<open>es os1 1 = lxs\<close>
+  \<open>outpu os1 1 = map (\<lambda> (d, t). (Inl d, t)) out_os1\<close>
+  \<open>input os2 1 = map (\<lambda> (d, t). (Inl d, t)) inp_os2\<close>
+  \<open>buf = out_os1 @ cbuf @ inp_os2\<close>
+  and
+  subgraph_inv:
+  \<open>(a, st1) = obtain_progress os1\<close>   
+  \<open>(b, st2) = obtain_progress os2\<close>
+  \<open>cgs = extract_progress 0 (edges sg) st1 @ extract_progress 1 (edges sg) st2\<close>
+  \<open>sg = subgraph_inv main_dt cgs c\<close>
+  \<open>c' = pt_tr sg\<close>
+  and
+  c_pts_inv:
+  \<open>c_pts c' (Loc 0 (Trg 1)) = {#}\<^sub>z\<close>
+  \<open>c_pts c' (Loc 0 (Src 1)) = zmset_of (mset (ocaps os1 1))\<close>
+  \<open>c_pts c' (Loc 1 (Trg 0)) = zmset_of (mset (map snd buf))\<close>
+  \<open>c_pts c' (Loc 1 (Src 1)) = zmset_of (mset (ocaps os2 1))\<close>
+  and
+  c_imp_inv:
+  \<open>front os2 1 \<le> frontier (c_imp c (Loc 1 (Trg 0)))\<close>
+
 shows 
   \<open>dataflow_op sg (inp_bt_op os1 (\<lambda> p. case p of Inl x \<Rightarrow> [] | Inr x \<Rightarrow> map (\<lambda> (d, t). Inr (Inl d, t)) cbuf) os2 f) \<approx>
-   map_op (\<lambda> p. (1, p)) (\<lambda> p. (1, p)) (source_op (\<lambda> p. outpu os2 1 @@- lmap (\<lambda> (d, t). (Inr d, t)) (lconcat (batch_fun_spec f lxs' buf caps))))\<close>
+   map_op (\<lambda> p. (1, p)) (\<lambda> p. (1, p)) (source_op (\<lambda> p. outpu os2 1 @@- lmap (\<lambda> (d, t). (Inr d, t)) (lconcat (batch_fun_spec f lxs buf caps))))\<close>
 
-
-  term outpos1
-  term buf
-  oops
-
+  term "ocaps os1 1"
 
 end
