dataplane/LList_Haskell_Setup.thy
@@ -1,0 +1,27 @@
+theory LList_Haskell_Setup
+
+imports
+  "Coinductive.Coinductive_List"
+  Nondeterministic_Dataflow.CSet_LList_Impl
+  "Timely_Infrastructure"
+begin
+
+(* code_printing code_module "Deter" \<rightharpoonup> (Haskell)
+  \<open>
+module Deter (cthe_elem, Cset (..) ) where
+
+newtype Cset a = Cset_of_llist [a];
+
+cthe_elem (Cset_of_llist xs) = Prelude.head xs;
+\<close>
+ *)
+
+
+
+(*    | constant sum_list \<rightharpoonup>
+    (Haskell) "sum"  *)
+(*   | constant fold \<rightharpoonup>
+    (Haskell) "(\\f xs x -> Prelude.foldl f x xs)"
+ *)
+
+end
